LeanSAT/AIG/CachedLemmas.lean
@@ -20,12 +20,17 @@ theorem denote_mkGate_cached {env : Env} {hl} {hr}
 /--
 `Env.mkGateCached` never shrinks the underlying AIG.
 -/
-theorem mkGateCached_le_size (lhs rhs : Nat) (linv rinv : Bool) (env : Env) hl hr
+theorem mkGateCached_le_size (env : Env) (lhs rhs : Nat) (linv rinv : Bool) hl hr
     : env.decls.size ≤ (env.mkGateCached lhs rhs linv rinv hl hr).env.decls.size := by
   dsimp [mkGateCached]
   split
   . simp
   . simp_arith
+
+theorem lt_of_lt_mkGateCached_size (entry : Entrypoint) (lhs rhs : Nat) (linv rinv : Bool) (hl) (hr) (h : x < entry.env.decls.size)
+    : x < (entry.env.mkGateCached lhs rhs linv rinv hl hr).env.decls.size := by
+  have := mkGateCached_le_size entry.env lhs rhs linv rinv hl hr
+  omega
 
 /--
 Reusing an `Env.Entrypoint` to build an additional gate will never invalidate the entry node of
@@ -39,10 +44,77 @@ theorem lt_mkGateCached_size (entry : Entrypoint) (lhs rhs : Nat) (linv rinv : B
   omega
 
 /--
+`mkGateCached` does not modify the input AIG upon a cache hit.
+-/
+theorem mkGateCached_hit_env (env : Env) (hcache : env.cache.find? (.gate lhs rhs linv rinv) = some gate) (hl) (hr) :
+    (env.mkGateCached lhs rhs linv rinv hl hr).env = env := by
+  simp only [mkGateCached]
+  split <;> simp_all
+
+/--
+`mkGateCached` pushes to the input AIG upon a cache miss.
+-/
+theorem mkGateCached_miss_env (env : Env) (hcache : env.cache.find? (.gate lhs rhs linv rinv) = none) (hl) (hr) :
+    (env.mkGateCached lhs rhs linv rinv hl hr).env.decls = env.decls.push (.gate lhs rhs linv rinv) := by
+  simp only [mkGateCached]
+  split <;> simp_all
+
+/--
+The AIG produced by `Env.mkGateCached` agrees with the input AIG on all indices that are valid for both.
+-/
+theorem mkGateCached_decl_eq idx (env : Env) (lhs rhs : Nat) (linv rinv : Bool)
+    {h : idx < env.decls.size} {hl} {hr} {hbound} :
+    (env.mkGateCached lhs rhs linv rinv hl hr).env.decls[idx]'hbound = env.decls[idx] := by
+  match hcache:env.cache.find? (.gate lhs rhs linv rinv) with
+  | some gate =>
+    have := mkGateCached_hit_env env hcache hl hr
+    simp [this]
+  | none =>
+    have := mkGateCached_miss_env env hcache hl hr
+    simp only [this, Array.get_push]
+    split
+    . rfl
+    . contradiction
+
+/--
+The input AIG to an `Env.mkGateCached` is a prefix to the output AIG.
+-/
+theorem mkGateCached_IsPrefix_env {env : Env} {hl} {hr} :
+    IsPrefix env.decls (env.mkGateCached lhs rhs lpol rpol hl hr).env.decls := by
+  apply IsPrefix.of
+  . intro idx h
+    apply mkGateCached_decl_eq
+  . apply mkGateCached_le_size
+
+@[simp]
+theorem denote_mkGateCached_entry (entry : Entrypoint) {hlbound} {hrbound} {h} :
+    ⟦(entry.env.mkGateCached lhs rhs lpol rpol hlbound hrbound).env, ⟨entry.start, h⟩, assign ⟧
+      =
+    ⟦entry, assign⟧ :=  by
+  apply denote.eq_of_env_eq
+  apply mkGateCached_IsPrefix_env
+
+@[simp]
+theorem denote_mkGateCached_lhs (entry : Entrypoint) {hlbound} {hrbound} {h} :
+    ⟦(entry.env.mkGateCached lhs rhs lpol rpol hlbound hrbound).env, ⟨lhs, h⟩, assign⟧
+      =
+    ⟦entry.env, ⟨lhs, hlbound⟩, assign⟧ :=  by
+  apply denote.go_eq_of_env_eq
+  apply mkGateCached_IsPrefix_env
+
+@[simp]
+theorem denote_mkGateCached_rhs (entry : Entrypoint) {hlbound} {hrbound} {h} :
+    ⟦(entry.env.mkGateCached lhs rhs lpol rpol hlbound hrbound).env, ⟨rhs, h⟩, assign⟧
+      =
+    ⟦entry.env, ⟨rhs, hrbound⟩, assign⟧ :=  by
+  apply denote.go_eq_of_env_eq
+  apply mkGateCached_IsPrefix_env
+
+/--
 The central equality theorem between `mkGateCached` and `mkGate`.
 -/
-theorem mkGateCached_eval_eq_mkGate_eval (lhs rhs : Nat) (linv rinv : Bool) (env : Env) (hl : lhs < env.decls.size)
-    (hr : rhs < env.decls.size) :
+@[simp]
+theorem mkGateCached_eval_eq_mkGate_eval {env : Env} {hl} {hr} :
     ⟦env.mkGateCached lhs rhs linv rinv hl hr, assign⟧ = ⟦env.mkGate lhs rhs linv rinv hl hr, assign⟧ := by
   simp only [mkGateCached]
   split
@@ -61,6 +133,38 @@ theorem denote_mkAtom_cached {env : Env} (h : env.cache.find? (.atom v) = some g
   split <;> simp_all
 
 /--
+`mkAtomCached` does not modify the input AIG upon a cache hit.
+-/
+theorem mkAtomCached_hit_env (env : Env) (hcache : env.cache.find? (.atom var) = some gate) :
+    (env.mkAtomCached var).env = env := by
+  simp only [mkAtomCached]
+  split <;> simp_all
+
+/--
+`mkAtomCached` pushes to the input AIG upon a cache miss.
+-/
+theorem mkAtomCached_miss_env (env : Env) (hcache : env.cache.find? (.atom var) = none) :
+    (env.mkAtomCached var).env.decls = env.decls.push (.atom var) := by
+  simp only [mkAtomCached]
+  split <;> simp_all
+
+/--
+The AIG produced by `Env.mkAtomCached` agrees with the input AIG on all indices that are valid for both.
+-/
+theorem mkAtomCached_decl_eq (env : Env) (var : Nat) (idx : Nat) {h : idx < env.decls.size} {hbound} :
+    (env.mkAtomCached var).env.decls[idx]'hbound = env.decls[idx] := by
+  match hcache:env.cache.find? (.atom var) with
+  | some gate =>
+    have := mkAtomCached_hit_env env hcache
+    simp [this]
+  | none =>
+    have := mkAtomCached_miss_env env hcache
+    simp only [this, Array.get_push]
+    split
+    . rfl
+    . contradiction
+
+/--
 `Env.mkAtomCached` never shrinks the underlying AIG.
 -/
 theorem mkAtomCached_le_size (env : Env) (var : Nat)
@@ -73,7 +177,8 @@ theorem mkAtomCached_le_size (env : Env) (var : Nat)
 /--
 The central equality theorem between `mkAtomCached` and `mkAtom`.
 -/
-theorem mkAtomCached_eval_eq_mkAtom_eval (var : Nat) (env : Env)
+@[simp]
+theorem mkAtomCached_eval_eq_mkAtom_eval {env : Env}
     : ⟦env.mkAtomCached var, assign⟧ = ⟦env.mkAtom var, assign⟧ := by
   simp only [mkAtomCached]
   split
@@ -92,6 +197,38 @@ theorem denote_mkConst_cached {env : Env} (h : env.cache.find? (.const b) = some
   split <;> simp_all
 
 /--
+`mkConstCached` does not modify the input AIG upon a cache hit.
+-/
+theorem mkConstCached_hit_env (env : Env) (hcache : env.cache.find? (.const val) = some gate) :
+    (env.mkConstCached val).env = env := by
+  simp only [mkConstCached]
+  split <;> simp_all
+
+/--
+`mkConstCached` pushes to the input AIG upon a cache miss.
+-/
+theorem mkConstCached_miss_env (env : Env) (hcache : env.cache.find? (.const val) = none) :
+    (env.mkConstCached val).env.decls = env.decls.push (.const val) := by
+  simp only [mkConstCached]
+  split <;> simp_all
+
+/--
+The AIG produced by `Env.mkConstCached` agrees with the input AIG on all indices that are valid for both.
+-/
+theorem mkConstCached_decl_eq (env : Env) (val : Bool) (idx : Nat) {h : idx < env.decls.size} {hbound} :
+    (env.mkConstCached val).env.decls[idx]'hbound = env.decls[idx] := by
+  match hcache:env.cache.find? (.const val) with
+  | some gate =>
+    have := mkConstCached_hit_env env hcache
+    simp [this]
+  | none =>
+    have := mkConstCached_miss_env env hcache
+    simp only [this, Array.get_push]
+    split
+    . rfl
+    . contradiction
+
+/--
 `Env.mkConstCached` never shrinks the underlying AIG.
 -/
 theorem mkConstCached_le_size (env : Env) (val : Bool)
@@ -100,6 +237,11 @@ theorem mkConstCached_le_size (env : Env) (val : Bool)
   split
   . simp
   . simp_arith
+
+theorem lt_of_lt_mkConstCached_size (entry : Entrypoint) (val : Bool) (h : x < entry.env.decls.size) :
+    x < (entry.env.mkConstCached val).env.decls.size := by
+  have := mkConstCached_le_size entry.env val
+  omega
 
 /--
 Reusing an `Env.Entrypoint` to build an additional constant will never invalidate the entry node of
@@ -111,10 +253,25 @@ theorem lt_mkConstCached_size (entry : Entrypoint) : entry.start < (entry.env.mk
     Env.mkConstCached_le_size _ _
   omega
 
+theorem mkConstCached_IsPrefix_env : IsPrefix env.decls (mkConstCached val env).env.decls := by
+  apply IsPrefix.of
+  . intro idx h
+    apply mkConstCached_decl_eq
+  . apply mkConstCached_le_size
+
+@[simp]
+theorem denote_mkConstCached_lt (entry : Entrypoint) {h} :
+    ⟦(entry.env.mkConstCached val).env, ⟨entry.start, h⟩, assign⟧
+      =
+    ⟦entry, assign⟧ := by
+  apply denote.eq_of_env_eq
+  apply mkConstCached_IsPrefix_env
+
 /--
 The central equality theorem between `mkConstCached` and `mkConst`.
 -/
-theorem mkConstCached_eval_eq_mkConst_eval (val : Bool) (env : Env)
+@[simp]
+theorem mkConstCached_eval_eq_mkConst_eval {env : Env}
     : ⟦env.mkConstCached val, assign⟧ = ⟦env.mkConst val, assign⟧ := by
   simp only [mkConstCached]
   split
